proofs/transform/eliminate_let.v
@@ -1,0 +1,1675 @@
+(*Eliminate let*)
+
+Require Import Alpha.
+Require Import Task.
+From Equations Require Import Equations.
+Set Bullet Behavior "Strict Subproofs".
+
+(*First version (not why3's)*)
+Section ElimLetAlt.
+
+Fixpoint elim_let_t (bt: bool) (bf: bool) (t: term) : term :=
+  match t with
+  | Tlet tm1 x tm2 => 
+    if bt then
+    safe_sub_t (elim_let_t bt bf tm1) x (elim_let_t bt bf tm2)
+    else Tlet (elim_let_t bt bf tm1) x (elim_let_t bt bf tm2)
+  | Tfun f tys tms => Tfun f tys (map (elim_let_t bt bf) tms)
+  | Tif f t1 t2 =>
+    Tif (elim_let_f bt bf f) (elim_let_t bt bf t1)
+      (elim_let_t bt bf t2)
+  | Tmatch tm ty ps =>
+    Tmatch (elim_let_t bt bf tm) ty
+      (map (fun x => (fst x, elim_let_t bt bf (snd x))) ps)
+  | Teps f v =>
+    Teps (elim_let_f bt bf f) v
+  | _ => t
+  end
+with elim_let_f (bt: bool) (bf: bool) (f: formula) : formula :=
+  match f with
+  | Fpred ps tys tms => Fpred ps tys (map (elim_let_t bt bf) tms)
+  | Fquant q v f => Fquant q v (elim_let_f bt bf f)
+  | Feq ty t1 t2 => Feq ty (elim_let_t bt bf t1) (elim_let_t bt bf t2)
+  | Fbinop b f1 f2 => Fbinop b (elim_let_f bt bf f1) (elim_let_f bt bf f2)
+  | Fnot f => Fnot (elim_let_f bt bf f)
+  | Flet tm1 v f =>
+    if bf then
+    safe_sub_f (elim_let_t bt bf tm1) v (elim_let_f bt bf f)
+    else Flet (elim_let_t bt bf tm1) v (elim_let_f bt bf f)
+  | Fif f1 f2 f3 => Fif (elim_let_f bt bf f1) (elim_let_f bt bf f2)
+    (elim_let_f bt bf f3)
+  | Fmatch tm ty ps =>
+    Fmatch (elim_let_t bt bf tm) ty
+      (map (fun x => (fst x, elim_let_f bt bf (snd x))) ps)
+  | _ => f
+  end.
+
+(*TODO: we should really generalize to some kind of mapping*)
+
+Lemma elim_let_typed gamma bt bf (t: term) (f: formula) :
+  (forall ty (Hty: term_has_type gamma t ty),
+    term_has_type gamma (elim_let_t bt bf t) ty) /\
+  (forall (Hty: formula_typed gamma f), formula_typed gamma (elim_let_f bt bf f)).
+Proof.
+  revert t f; apply term_formula_ind; simpl; auto; intros;
+  inversion Hty; subst; try solve[constructor; auto].
+  - constructor; auto. rewrite map_length; auto.
+    assert (Hlen: length (map (ty_subst (s_params f1) l) (s_args f1)) =
+      length l1) by (rewrite map_length; auto).
+    clear -H10 Hlen H.
+    generalize dependent l1.
+    induction (map (ty_subst (s_params f1) l) (s_args f1)); simpl;
+    intros;
+    destruct l1; inversion Hlen; auto.
+    inversion H; subst. inversion H10; subst.
+    constructor; auto.
+  - destruct v as [x xty]; simpl in *.
+    destruct bt. 
+    + apply safe_sub_t_typed; auto.
+    + constructor; auto.
+  - constructor; auto; [| | rewrite null_map; auto].
+    + intros x. rewrite in_map_iff.
+      intros [y [Hx Hiny]]; subst; simpl; auto.
+    + clear -H9 H0. induction ps; simpl in *; auto;
+      intros.
+      inversion H0; subst.
+      destruct H; subst; simpl; auto.
+  - constructor; auto. rewrite map_length; auto.
+    assert (Hlen: length (map (ty_subst (s_params p) tys) (s_args p)) =
+      length tms) by (rewrite map_length; auto).
+    clear -H8 Hlen H.
+    generalize dependent tms.
+    induction (map (ty_subst (s_params p) tys) (s_args p)); simpl;
+    intros;
+    destruct tms; inversion Hlen; auto.
+    inversion H; subst. inversion H8; subst.
+    constructor; auto.
+  - destruct v as [x xty]; simpl in *.
+    destruct bf. 
+    + apply safe_sub_f_typed; auto.
+    + constructor; auto.
+  - constructor; auto; [| | rewrite null_map; auto].
+    + intros x. rewrite in_map_iff.
+      intros [y [Hx Hiny]]; subst; simpl; auto.
+    + clear -H8 H0. induction ps; simpl in *; auto;
+      intros.
+      inversion H0; subst.
+      destruct H; subst; simpl; auto.
+Qed.
+
+Definition elim_let_t_typed bt bf t gamma := proj_tm 
+  (elim_let_typed gamma bt bf) t.
+Definition elim_let_f_typed bt bf f gamma := proj_fmla 
+  (elim_let_typed gamma bt bf) f.
+
+(*Then prove free vars*)
+
+Lemma sublist_refl {A: Type} (l: list A):
+  sublist l l.
+Proof.
+  unfold sublist. auto.
+Qed.
+
+Lemma sublist_big_union {A B: Type} 
+  (eq_dec: forall (x y: A), {x=y} + {x<>y})
+  (f: B -> list A) (l: list B) (g: B -> B):
+  Forall (fun x => sublist (f (g x)) (f x)) l ->
+  sublist (big_union eq_dec f (map g l)) (big_union eq_dec f l).
+Proof.
+  intros.
+  unfold sublist.
+  intros. simpl_set.
+  rewrite Forall_forall in H.
+  destruct H0 as [y [Hiny Hinx]].
+  rewrite in_map_iff in Hiny.
+  destruct Hiny as [z [Hy Hinz]]; subst.
+  exists z. split; auto.
+  apply H in Hinz.
+  apply Hinz; auto.
+Qed.
+
+Lemma sublist_union {A: Type} (eq_dec: forall (x y: A), {x=y}+{x<>y})
+  (l1 l2 l3 l4: list A):
+  sublist l1 l2 ->
+  sublist l3 l4 ->
+  sublist (union eq_dec l1 l3) (union eq_dec l2 l4).
+Proof.
+  unfold sublist. intros. simpl_set.
+  destruct H1; auto.
+Qed.
+
+Lemma sublist_remove {A: Type} (eq_dec: forall (x y: A), {x=y}+{x<>y})
+  v l1 l2:
+  sublist l1 l2 ->
+  sublist (remove eq_dec v l1) (remove eq_dec v l2).
+Proof.
+  unfold sublist; intros; simpl_set; destruct_all; split; auto.
+Qed.
+
+Lemma sublist_remove_all  {A: Type} (eq_dec: forall (x y: A), {x=y}+{x<>y})
+  l1 l2 l3:
+  sublist l2 l3 ->
+  sublist (remove_all eq_dec l1 l2) (remove_all eq_dec l1 l3).
+Proof.
+  unfold sublist; intros; simpl_set; destruct_all; auto.
+Qed.
+
+(*Need sublist (not eq) because the var to sub may not
+  be in the term*)
+Lemma elim_let_fv bt bf (t: term) (f: formula) :
+  (sublist (tm_fv (elim_let_t bt bf t)) (tm_fv t)) /\
+  (sublist (fmla_fv (elim_let_f bt bf f)) (fmla_fv f)).
+Proof.
+  revert t f; apply term_formula_ind; simpl; intros; auto;
+  try apply sublist_refl.
+  - apply sublist_big_union; auto.
+  - destruct bt; simpl.
+    + (*Need to know if var to sub appears freely in term or not*) 
+      destruct (in_dec vsymbol_eq_dec v  (tm_fv (elim_let_t true bf tm2))).
+      * unfold sublist. intros x.
+        rewrite safe_sub_t_fv; auto; simpl_set. intros;
+        destruct_all; auto.
+      * rewrite safe_sub_t_notin; auto.
+        unfold sublist. intros.
+        simpl_set.
+        right. split; auto.
+        intro C; subst; contradiction.
+    + apply sublist_union; auto.
+      apply sublist_remove; auto.
+  - repeat (apply sublist_union; auto).
+  - apply sublist_union; auto.
+    apply sublist_big_union; auto.
+    rewrite Forall_map in H0; revert H0. simpl.
+    apply Forall_impl; intros.
+    apply sublist_remove_all; auto.
+  - apply sublist_remove; auto.
+  - apply sublist_big_union; auto.
+  - apply sublist_remove; auto.
+  - apply sublist_union; auto.
+  - apply sublist_union; auto.
+  - destruct bf; simpl.
+    + destruct (in_dec vsymbol_eq_dec v  (fmla_fv (elim_let_f bt true f))).
+      * unfold sublist. intros x.
+        rewrite safe_sub_f_fv; auto; simpl_set. intros;
+        destruct_all; auto.
+      * rewrite safe_sub_f_notin; auto.
+        unfold sublist. intros.
+        simpl_set.
+        right. split; auto.
+        intro C; subst; contradiction.
+    + apply sublist_union; auto.
+      apply sublist_remove; auto.
+  - repeat (apply sublist_union; auto).
+  - apply sublist_union; auto.
+    apply sublist_big_union; auto.
+    rewrite Forall_map in H0.
+    revert H0. apply Forall_impl.
+    intros. apply sublist_remove_all; auto.
+Qed.
+
+Definition elim_let_f_fv bt bf f :=
+  proj_fmla (elim_let_fv bt bf) f.
+
+(*Finally, prove that the semantics are preserved*)
+Section Rep.
+
+Context {gamma: context} (gamma_valid: valid_context gamma) 
+  (pd: pi_dom) (vt: val_typevar) (pf: pi_funpred gamma_valid pd).
+
+Lemma elim_let_rep bt bf t f:
+  (forall vv ty (Hty1: term_has_type gamma t ty) 
+    (Hty2: term_has_type gamma (elim_let_t bt bf t) ty),
+    term_rep gamma_valid pd vt pf vv (elim_let_t bt bf t) ty Hty2 =
+    term_rep gamma_valid pd vt pf vv t ty Hty1) /\
+  (forall vv (Hty1: formula_typed gamma f) 
+    (Hty2: formula_typed gamma (elim_let_f bt bf f)),
+    formula_rep gamma_valid pd vt pf vv (elim_let_f bt bf f) Hty2 =
+    formula_rep gamma_valid pd vt pf vv f Hty1).
+Proof.
+  revert t f; apply term_formula_ind; intros;
+  try solve[simpl; apply term_rep_irrel];
+  try solve[simpl_rep_full; apply fmla_rep_irrel];
+  try reflexivity;
+  simpl in *; simpl_rep_full.
+  - (*TODO: need better way to do this - maybe sep
+      extensionality lemma for these*)
+    assert (ty_fun_ind_ret Hty2 = ty_fun_ind_ret Hty1).
+      apply UIP_dec. apply vty_eq_dec.
+    rewrite H0. f_equal. f_equal. apply UIP_dec. apply sort_eq_dec.
+    f_equal. apply get_arg_list_ext; rewrite map_length; auto.
+    intros.
+    rewrite Forall_forall in H.
+    revert Hty0.
+    rewrite map_nth_inbound with(d2:=tm_d); auto; intros.
+    apply H. apply nth_In; auto.
+  - destruct bt.
+    + destruct v as [x xty].
+      erewrite safe_sub_t_rep, H, H0.
+      reflexivity.
+      Unshelve.
+      all: inversion Hty1; subst;
+      apply elim_let_t_typed; auto.
+    + simpl_rep_full. erewrite H, H0. reflexivity.
+  - erewrite H, H0, H1; reflexivity.
+  - iter_match_gen Hty1 Htm1 Hpat1 Hty1.
+    iter_match_gen Hty2 Htm2 Hpat2 Hty2.
+    induction ps; simpl; intros; auto.
+    simpl in *. destruct a as [p1 t1];
+    simpl in *.
+    rewrite H with(Hty1:=Hty1) at 1.
+    rewrite match_val_single_irrel with (Hval2:=(Forall_inv Hpat1)).
+    simpl.
+    inversion H0; subst.
+    case_match_goal; auto.
+  - f_equal.
+    apply functional_extensionality_dep; intros.
+    assert ((proj2' (ty_eps_inv Hty2)) = (proj2' (ty_eps_inv Hty1))). {
+      apply UIP_dec. apply vty_eq_dec.
+    }
+    erewrite H0, H. reflexivity.
+  - f_equal. apply get_arg_list_ext; rewrite map_length; auto;
+    intros. revert Hty0.
+    rewrite map_nth_inbound with(d2:=tm_d); auto; intros.
+    rewrite Forall_forall in H; apply H; auto.
+    apply nth_In; auto.
+  - destruct q; simpl_rep_full; apply all_dec_eq;
+    split; [intros Hd d | intros Hd d | intros [d Hd]; exists d |
+    intros [d Hd]; exists d]; try (erewrite H; apply Hd);
+    erewrite <- H; apply Hd.
+  - erewrite H, H0; reflexivity.
+  - erewrite H, H0; reflexivity.
+  - erewrite H; reflexivity.
+  - destruct bf.
+    + destruct v as [x xty].
+      erewrite safe_sub_f_rep, H, H0.
+      reflexivity.
+      Unshelve.
+      all: inversion Hty1; subst.
+      apply elim_let_t_typed; auto.
+      apply elim_let_f_typed; auto.
+    + simpl_rep_full.
+      erewrite H, H0. reflexivity.
+  - erewrite H, H0, H1; reflexivity.
+  - iter_match_gen Hty1 Htm1 Hpat1 Hty1.
+    iter_match_gen Hty2 Htm2 Hpat2 Hty2.
+    induction ps; simpl; intros; auto.
+    destruct a as [p1 t1]; simpl in *.
+    rewrite H with(Hty1:=Hty1) at 1.
+    rewrite match_val_single_irrel with (Hval2:=(Forall_inv Hpat1)).
+    simpl.
+    inversion H0; subst.
+    case_match_goal; auto.
+Qed.
+  
+Definition elim_let_f_rep bt bf f :=
+  proj_fmla (elim_let_rep bt bf) f.
+  
+
+End Rep.
+
+(*Define the transformation*)
+Definition eliminate_let_term (gamma: context) : trans gamma :=
+  trans_goal gamma (elim_let_f true false).
+  
+Definition eliminate_let_fmla (gamma: context) : trans gamma :=
+  trans_goal gamma (elim_let_f false true).
+
+Definition eliminate_let (gamma: context) : trans gamma :=
+  trans_goal gamma (elim_let_f true true).
+
+(*Now we prove soundness*)
+Lemma eliminate_let_sound_gen (gamma: context) :
+  forall b1 b2,
+  sound_trans (trans_goal gamma (elim_let_f b1 b2)).
+Proof.
+  intros.
+  apply trans_goal_sound.
+  intros. split_all.
+  - apply elim_let_f_typed; auto.
+  - apply elim_let_f_fv.
+  - intros. erewrite elim_let_f_rep in H.
+    apply H.
+Qed.
+
+Theorem eliminate_let_term_sound gamma:
+  sound_trans (eliminate_let_term gamma).
+Proof.
+  apply eliminate_let_sound_gen.
+Qed.
+
+Theorem eliminate_let_fmla_sound gamma:
+  sound_trans (eliminate_let_fmla gamma).
+Proof.
+  apply eliminate_let_sound_gen.
+Qed.
+
+Theorem elim_let_sound gamma:
+  sound_trans (eliminate_let gamma).
+Proof.
+  apply eliminate_let_sound_gen.
+Qed.
+
+End ElimLetAlt.
+
+(*The Why3 implementation is a lot more difficult to deal with,
+  though it is arguably a bit more "natural" - it more closely
+  mirrors what a human might do.
+  The main difference is that it does f(t2[f(t1) / x])
+  instead of (f(t2))[f(t1) /x]. This induces many difficulties:
+  1. It is not structurally decreasing, so we cannot write it as
+    a Fixpoint.
+  2. The termination measure is actually very tricky. One measure
+    that works is a lexicographic order (number of lets, size of term).
+    Formalizing this takes some work: we need to define these metrics.
+  3. Even with the termination measure, Equations (and Program, and
+    Function) do not allow well-founded mutual recursion. So we have
+    to awkwardly encode our function as a single dependently typed
+    function.
+  4. For mapping over a list recursively, we need to use a dependent 
+    map function, or else we lose information in the Equations
+    obligations.
+  5. Finally, in the Tlet/Flet cases, the number of lets (the first
+    measure) only decreases if the term we substitute has no lets
+    in it. Since this is a recursive call, we need the return
+    type of our function to be a sigma type encoding this info.
+*)
+Require Import Coq.Relations.Relation_Operators.
+Section ElimLetWhy3.
+
+(*To start, we define the size of a term/formula*)
+Fixpoint tm_size (t: term) : nat :=
+  match t with
+  | Tconst c => 0
+  | Tvar _ => 0
+  | Tfun _ _ tms => 1 + sum (map tm_size tms)
+  | Tlet t1 _ t2 => 1 + tm_size t1 + tm_size t2
+  | Tif f t1 t2 => 1+ fmla_size f + tm_size t1 + tm_size t2
+  | Tmatch tm _ ps =>
+    1 + tm_size tm + sum (map (fun x => tm_size (snd x)) ps)
+  | Teps f _ => 1 + fmla_size f
+  end
+with fmla_size (f: formula) : nat :=
+  match f with
+  | Fpred _ _ tms => 1 + sum (map tm_size tms)
+  | Fquant _ _ f => 1 + fmla_size f
+  | Feq _ t1 t2 => 1 + tm_size t1 + tm_size t2
+  | Fbinop _ f1 f2 => 1 + fmla_size f1 + fmla_size f2
+  | Fnot f => 1 + fmla_size f
+  | Ftrue => 0
+  | Ffalse => 0
+  | Flet tm _ f => 1 + tm_size tm + fmla_size f
+  | Fif f1 f2 f3 => 1 + fmla_size f1 + fmla_size f2 + fmla_size f3
+  | Fmatch tm _ ps =>
+    1 + tm_size tm + sum (map (fun x => fmla_size (snd x)) ps)
+  end.
+
+Variable bt: bool.
+Variable bf: bool.
+
+(*Count the number of "lets" in a term/formula*)
+Fixpoint count_let_t (t: term) : nat :=
+  match t with
+  | Tfun _ _ tms => sum (map count_let_t tms)
+  | Tlet t1 v t2 =>
+    count_let_t t1 + (if bt then 1 else 0) +
+    count_let_t t2
+  | Tif f t1 t2 => count_let_f f + count_let_t t1 + count_let_t t2
+  | Tvar v => 0
+  | Tconst _ => 0
+  | Teps f v => count_let_f f
+  | Tmatch t _ ps => count_let_t t +
+    sum (map (fun p => count_let_t (snd p)) ps)
+  end
+with count_let_f (f: formula) : nat :=
+  match f with
+  | Fpred _ _ tms => sum (map count_let_t tms)
+  | Fquant _ v f => count_let_f f
+  | Fbinop _ f1 f2 => count_let_f f1 + count_let_f f2
+  | Feq _ t1 t2 => count_let_t t1 + count_let_t t2
+  | Fnot f => count_let_f f
+  | Flet t v f => count_let_t t + (if bf then 1 else 0) +
+    count_let_f f
+  | Fif f1 f2 f3 => count_let_f f1 + count_let_f f2 +
+    count_let_f f3
+  | Fmatch t _ ps => count_let_t t +
+    sum (map (fun p => count_let_f (snd p)) ps)
+  | Ftrue => 0
+  | Ffalse => 0
+  end.
+
+(*Build a lexicographic order based on 2 nat functions*)
+
+(*First, generic*)
+Section Lex.
+
+Context {A: Type} (r1 r2: A -> nat).
+
+Definition lexnat (x y: A): Prop :=
+  slexprod nat nat lt lt (r1 x, r2 x) (r1 y, r2 y).
+
+Lemma lexnat_wf: well_founded lexnat.
+Proof.
+  unfold lexnat.
+  unfold well_founded.
+  intros.
+  apply Inverse_Image.Acc_inverse_image.
+  apply Lexicographic_Product.wf_slexprod; auto;
+  apply Wf_nat.lt_wf.
+Defined.
+
+End Lex.
+
+(*The bundled types we need to eliminate mutual recursion*)
+
+Definition tm_fmla := Either term formula.
+Definition tm_fmla_ty (x: tm_fmla) : Type :=
+  match x with
+  | Left _ => term
+  | Right _ => formula
+  end.
+Definition tm_fmla_size (x: tm_fmla) : nat :=
+  match x with
+  | Left t => tm_size t
+  | Right f => fmla_size f
+  end.
+Definition tm_fmla_count_let (x: tm_fmla) : nat :=
+  match x with
+  | Left t => count_let_t t
+  | Right f => count_let_f f
+  end.
+
+Arguments Left {_} {_}.
+Arguments Right {_} {_}.
+
+Definition elim_let_rel: tm_fmla -> tm_fmla -> Prop :=
+  lexnat tm_fmla_count_let tm_fmla_size.
+
+Definition elim_let_rel_wf : well_founded elim_let_rel :=
+  lexnat_wf _ _.
+
+(*Dependent mapping over a list*)
+
+
+(*Inspired by Equations/examples/RoseTree.v*)
+
+Definition map_In {A B: Type} (l: list A) 
+  (f: forall (x: A), In x l -> B) : list B :=
+  dep_map f l (all_in_refl l).
+
+Lemma dep_map_length {A B: Type} {P: A -> Prop} 
+  (f: forall x: A, P x -> B) (l: list A) (Hall: Forall P l):
+  length (dep_map f l Hall) = length l.
+Proof.
+  revert Hall.
+  induction l; simpl; intros; auto.
+Qed.
+
+Lemma dep_map_nth {A B: Type} {P: A -> Prop}
+(f: forall x: A, P x -> B) (l: list A) (Hall: Forall P l)
+(i: nat) (d1: A) (d2: B) (Hnth: P (nth i l d1)):
+i < length l ->
+nth i (dep_map f l Hall) d2 =
+f (nth i l d1) Hnth.
+Proof.
+  revert i Hall Hnth. induction l; simpl; intros; auto.
+  - lia.
+  - destruct i. f_equal. apply proof_irrel.
+    apply IHl. lia.
+Qed.
+
+Lemma map_In_spec {A B : Type} (f : A -> B) (l : list A) :
+  map_In l (fun (x : A) (_ : In x l) => f x) = map f l.
+Proof.
+  (*This is very dumb, but we need an A*)
+  destruct l; auto.
+  remember (a :: l) as l'.
+  unfold map_In.
+  apply list_eq_ext'; rewrite dep_map_length; [rewrite map_length |]; auto.
+  intros n d Hn.
+  erewrite dep_map_nth with(d1:=a); auto; [|apply nth_In; auto].
+  rewrite map_nth_inbound with(d2:=a); auto.
+Qed.
+
+Lemma in_map_In_iff {A B: Type} (l: list A)
+  (f: forall (x: A), In x l -> B) (y: B):
+  In y (map_In l f) <-> exists x Hin, f x Hin = y.
+Proof.
+  unfold map_In. split; intros.
+  - apply dep_map_in in H.
+    destruct H as [x [H [Hinx Hy]]]; subst; exists x; exists H; auto.
+  - destruct H as [x [Hin Hy]]; subst.
+    assert (Hinx:=Hin).
+    apply in_dep_map with(f:=f)(Hall:=all_in_refl l) in Hinx.
+    destruct Hinx as [Hin' Hinx].
+    assert (Hin = Hin') by apply proof_irrel.
+    subst; auto.
+Qed.
+
+(*TODO: proof obligations about our measures*)
+Section ProofObligations.
+
+Lemma in_sum_le l x:
+  In x l ->
+  x <= sum l.
+Proof.
+  induction l; simpl; intros; destruct H; subst; auto;
+  try lia.
+  apply IHl in H; lia.
+Qed.
+
+(*sub_t relation with count_let_t*)
+
+Lemma count_let_sub tm x (Htm: count_let_t tm = 0) t f:
+  count_let_t (sub_t tm x t) = count_let_t t /\
+  count_let_f (sub_f tm x f) = count_let_f f.
+Proof.
+  revert t f; apply term_formula_ind; simpl; intros; auto.
+  - vsym_eq x v.
+  - f_equal. induction l1; simpl; auto.
+    inversion H; subst; auto. rewrite H2, IHl1; auto.
+  - rewrite H. destruct bt; auto; vsym_eq x v.
+  - rewrite H. f_equal. f_equal.
+    induction ps; simpl in *; auto.
+    inversion H0; subst.
+    rewrite IHps; auto.
+    destruct (in_bool vsymbol_eq_dec x (pat_fv (fst a))); simpl; auto.
+    rewrite H3; auto.
+  - vsym_eq x v.
+  - f_equal. induction tms; simpl; auto.
+    inversion H; subst; auto. rewrite H2, IHtms; auto.
+  - vsym_eq x v.
+  - rewrite H. destruct bf; auto; vsym_eq x v.
+  - rewrite H. f_equal. f_equal.
+    induction ps; simpl in *; auto.
+    inversion H0; subst.
+    rewrite IHps; auto.
+    destruct (in_bool vsymbol_eq_dec x (pat_fv (fst a))); simpl; auto.
+    rewrite H3; auto.
+Qed.
+
+Definition count_let_sub_t tm x t Htm :=
+  proj_tm (count_let_sub tm x Htm) t.
+Definition count_let_sub_f tm x f Htm :=
+  proj_fmla (count_let_sub tm x Htm) f.
+
+(*count_let is preserved by [shape]*)
+Lemma count_let_shape t1 f1:
+  (forall t2 (Heq: shape_t t1 t2),
+    count_let_t t1 = count_let_t t2) /\
+  (forall f2 (Heq: shape_f f1 f2),
+    count_let_f f1 = count_let_f f2).
+Proof.
+  revert t1 f1; apply term_formula_ind; simpl; intros; auto.
+  - alpha_case t2 Heq; auto.
+  - alpha_case t2 Heq; auto.
+  - alpha_case t2 Heq. bool_hyps.
+    f_equal.
+    nested_ind_case.
+    rewrite all2_cons in H1. bool_hyps.
+    erewrite IHl1, Hp; try reflexivity; auto.
+  - alpha_case t2 Heq. bool_hyps.
+    rewrite (H _ H1), (H0 _ H2); auto.
+  - alpha_case t0 Heq. bool_hyps.
+    rewrite (H _ H2), (H0 _ H4), (H1 _ H3); auto.
+  - alpha_case t2 Heq. bool_hyps.
+    rewrite (H _ H1); auto. f_equal. f_equal.
+    nested_ind_case.
+    rewrite all2_cons in H2.
+    bool_hyps.
+    rewrite (Hp _ H7), (IHps Hforall l); auto.
+  - alpha_case t2 Heq. apply H; auto.
+  - alpha_case f2 Heq.  bool_hyps.
+    f_equal.
+    nested_ind_case.
+    rewrite all2_cons in H1. bool_hyps.
+    erewrite IHtms, Hp; try reflexivity; auto.
+  - alpha_case f2 Heq. bool_hyps. apply H; auto.
+  - alpha_case f2 Heq. bool_hyps.
+    rewrite (H _ H3), (H0 _ H2); auto.
+  - alpha_case f0 Heq. bool_hyps.
+    rewrite (H _ H3), (H0 _ H2); auto.
+  - alpha_case f2 Heq. apply H; auto.
+  - alpha_case f2 Heq; auto.
+  - alpha_case f2 Heq; auto.
+  - alpha_case f2 Heq; bool_hyps.
+    rewrite (H _ H1), (H0 _ H2); auto.
+  - alpha_case f0 Heq. bool_hyps.
+    rewrite (H _ H2), (H0 _ H4), (H1 _ H3); auto.
+  - alpha_case f2 Heq. bool_hyps.
+    rewrite (H _ H1); auto. f_equal. f_equal.
+    nested_ind_case.
+    rewrite all2_cons in H2.
+    bool_hyps.
+    rewrite (Hp _ H7), (IHps Hforall l); auto.
+Qed.
+
+Definition count_let_shape_t t1 := proj_tm count_let_shape t1.
+Definition count_let_shape_f f1 := proj_fmla count_let_shape f1.
+
+(*And thus, this applies to [safe_sub]*)
+Lemma count_let_safe_sub_t tm x t (Htm: count_let_t tm = 0):
+  count_let_t (safe_sub_t tm x t) = count_let_t t.
+Proof.
+  unfold safe_sub_t.
+  destruct (in_bool vsymbol_eq_dec x (tm_fv t)); auto.
+  rewrite count_let_sub_t; auto.
+  destruct (existsb (fun x0 : vsymbol => in_bool vsymbol_eq_dec x0 (tm_bnd t)) (tm_fv tm)); auto.
+  apply count_let_shape_t.
+  apply alpha_shape_t with(vars:=nil).
+  rewrite a_equiv_t_sym.
+  apply a_convert_t_equiv.
+Qed.
+
+Lemma count_let_safe_sub_f tm x f (Htm: count_let_t tm = 0):
+  count_let_f (safe_sub_f tm x f) = count_let_f f.
+Proof.
+  unfold safe_sub_f.
+  destruct (in_bool vsymbol_eq_dec x (fmla_fv f)); auto.
+  rewrite count_let_sub_f; auto.
+  destruct (existsb (fun x0 : vsymbol => in_bool vsymbol_eq_dec x0 (fmla_bnd f)) (tm_fv tm)); auto.
+  apply count_let_shape_f.
+  apply alpha_shape_f with(vars:=nil).
+  rewrite a_equiv_f_sym.
+  apply a_convert_f_equiv.
+Qed.
+
+
+Lemma sum_0 l:
+  sum l = 0 <-> Forall (fun x => x = 0) l.
+Proof.
+  induction l; simpl; intros; split; intros; auto.
+  - constructor. lia. apply IHl; lia.
+  - inversion H; subst. rewrite IHl; auto.
+Qed.
+
+
+End ProofObligations.
+
+
+(*Now we can write the Equations function*)
+
+(*TODO: remove*)
+
+(*Not binding or type safe*)
+Definition t_map (f1: term -> term) (f2: formula -> formula) 
+  (t: term): term :=
+  match t with
+  | Tfun f vs tms => Tfun f vs (map_In tms (fun x H => f1 x))
+  | Tlet t1 v t2 => Tlet (f1 t1) v (f1 t2)
+  | Tif f t1 t2 => Tif (f2 f) (f1 t1) (f1 t2)
+  | Tmatch tm ty ps => Tmatch (f1 tm) ty 
+      (map (fun x => (fst x, f1 (snd x))) ps)
+  | Teps f v => Teps (f2 f) v
+  | _ => t
+  end.
+
+Definition f_map (f1: term -> term) (f2: formula -> formula) 
+  (f: formula): formula :=
+  match f with
+  | Fpred p tys tms => Fpred p tys (map f1 tms)
+  | Fquant q x f => Fquant q x (f2 f)
+  | Feq ty t1 t2 => Feq ty (f1 t1) (f1 t2)
+  | Fbinop b fa fb => Fbinop b (f2 fa) (f2 fb)
+  | Fnot f => Fnot (f2 f)
+  | Flet t v f => Flet (f1 t) v (f2 f)
+  | Fif fa fb fc => Fif (f2 fa) (f2 fb) (f2 fc)
+  | Fmatch tm ty ps => Fmatch (f1 tm) ty
+  (map (fun x => (fst x, f2 (snd x))) ps)
+  | _ => f
+  end.
+
+Instance elim_let_rel_wf':
+WellFounded
+        (Telescopes.tele_measure (Telescopes.tip tm_fmla) (Either term formula)
+           (fun x : tm_fmla => x) elim_let_rel).
+Proof.
+  apply elim_let_rel_wf.
+  Defined.
+
+Ltac destruct_sig :=
+  repeat match goal with
+  | |- context [(proj1_sig ?x)] => destruct x; simpl
+  end; simpl in *; try lia; auto.
+
+Obligation Tactic := intros; try(unfold elim_let_rel, lexnat); simpl;
+destruct_sig.
+
+Definition tm_fmla_count_let' {x: tm_fmla} (y: tm_fmla_ty x) : nat :=
+  match x as x' return tm_fmla_ty x' -> nat with
+  | Left _ => fun t => count_let_t t
+  | Right _ => fun f => count_let_f f
+  end y.
+
+
+
+Equations elim_let_tm_fmla (x: tm_fmla) : 
+  { r: tm_fmla_ty x | tm_fmla_count_let' r = 0}
+  by wf x elim_let_rel :=
+elim_let_tm_fmla (Left (Tlet tm1 x tm2)) =>
+  let t1 := proj1_sig (elim_let_tm_fmla (Left tm1)) in
+  (*Need to retain info about bt in proof*)
+  match bt as b return bt = b -> 
+  {r : tm_fmla_ty (Left (Tlet tm1 x tm2)) | tm_fmla_count_let' r = 0} with
+  (*Why we need this: not structurally recursive*)
+  | true => fun Hb => 
+     elim_let_tm_fmla (Left (safe_sub_t t1 x tm2))
+  | false => fun Hb => 
+    exist _ (Tlet t1 x (proj1_sig (elim_let_tm_fmla (Left tm2)))) _
+  end eq_refl ;
+elim_let_tm_fmla (Left (Tconst c)) := exist _ (Tconst c) eq_refl;
+elim_let_tm_fmla (Left (Tvar v)) := exist _ (Tvar v) eq_refl;
+elim_let_tm_fmla (Left (Tfun f tys tms)) :=
+  exist _ (Tfun f tys (map_In tms 
+    (fun x H => proj1_sig (elim_let_tm_fmla (Left x))))) _;
+elim_let_tm_fmla (Left (Tif f t1 t2)) :=
+  exist _ (Tif (proj1_sig (elim_let_tm_fmla (Right f))) 
+    (proj1_sig (elim_let_tm_fmla (Left t1)))
+    (proj1_sig (elim_let_tm_fmla (Left t2)))) _;
+elim_let_tm_fmla (Left t) := exist _ (t_map 
+  (fun x => proj1_sig (elim_let_tm_fmla (Left x)))
+  (fun x => proj1_sig (elim_let_tm_fmla (Right x))) t) _;
+elim_let_tm_fmla (Right (Flet t x f)) =>
+  let t1 := proj1_sig (elim_let_tm_fmla (Left t)) in
+  (*Need to retain info about bt in proof*)
+  match bf as b return bf = b -> 
+  {r : tm_fmla_ty (Right (Flet t x f)) | tm_fmla_count_let' r = 0} with
+  (*Why we need this: not structurally recursive*)
+  | true => fun Hb => 
+    elim_let_tm_fmla (Right (safe_sub_f t1 x f))
+  | false => fun Hb => 
+    exist _ (Flet t1 x (proj1_sig (elim_let_tm_fmla (Right f)))) _
+  end eq_refl ;
+elim_let_tm_fmla (Right f) := exist _ (f_map 
+(fun x => proj1_sig (elim_let_tm_fmla (Left x)))
+(fun x => proj1_sig (elim_let_tm_fmla (Right x))) f) _.
+Next Obligation.
+(*Tfun termination*)
+(*Because of [map_In], we have the hypothesis we need*)
+assert (count_let_t x <= sum (map count_let_t tms)). {
+  apply in_sum_le; rewrite in_map_iff. exists x; auto.
+}
+apply Lt.le_lt_or_eq_stt in H0.
+destruct H0.
+- apply left_slex; auto.
+- rewrite H0. apply right_slex.
+  apply Arith_prebase.le_lt_n_Sm_stt.
+  apply in_sum_le.
+  rewrite in_map_iff; exists x; auto.
+Defined.
+Next Obligation.
+(*Tfun number of lets*)
+apply sum_0.
+rewrite Forall_forall. intros.
+rewrite in_map_iff in H.
+destruct H as [t [Hx Hint]]; subst.
+rewrite in_map_In_iff in Hint.
+destruct Hint as [x [Hinx Ht]]; subst.
+destruct_sig.
+Defined.
+Next Obligation.
+(*First let (t1) termination*)
+destruct bt; simpl.
+- apply left_slex. (*TODO: avoid lia maybe*) lia.
+- destruct (count_let_t tm2).
+  + rewrite !Nat.add_0_r. apply right_slex.
+    lia.
+  + apply left_slex; lia.
+Defined.
+Next Obligation.
+(*Hard one: the non-structurally-recursive let call*)
+rewrite Hb. (*We need info about bt*)
+(*Here, we need the info from the dependent type*)
+rewrite count_let_safe_sub_t.
+- apply left_slex. lia.
+- subst t1. simpl.
+  destruct ((elim_let_tm_fmla (Left tm1) 
+    (elim_let_tm_fmla_obligations_obligation_3 tm1 x tm2)));
+  simpl; auto.
+Defined.
+Next Obligation.
+(*The other let case (bt false)*)
+rewrite Hb.
+destruct (count_let_t tm1).
+- simpl. apply right_slex. lia.
+- apply left_slex; lia.
+Defined.
+Next Obligation.
+(*bt=false number of lets*)
+rewrite Hb at 1.
+rewrite Nat.add_0_r.
+subst t1; simpl.
+destruct_sig.
+Defined.
+Next Obligation.
+(*Termination for Tif - case 1*)
+rewrite <- Nat.add_assoc.
+destruct (count_let_t t1 + count_let_t t2);
+[rewrite Nat.add_0_r; apply right_slex| apply left_slex]; lia.
+Defined.
+Next Obligation.
+(*Tif termination 2*)
+rewrite (Nat.add_comm _ (count_let_t t1)), <- Nat.add_assoc.
+destruct (count_let_f f + count_let_t t2);
+[rewrite Nat.add_0_r; apply right_slex | apply left_slex]; lia.
+Defined.
+Next Obligation.
+(*Tif termination 3*)
+destruct (count_let_f f + count_let_t t1);
+[apply right_slex | apply left_slex]; lia.
+Defined.
+Next Obligation.
+(*Tmatch termination 1*)
+(*TODO: fix program, no map*)
+
+
+(*ALL BELOW IS OLD*)
+  
+
+
+(*Eliminate lets from terms and/or formulas by using 
+  (safe) substitution*)
+
+
+(*This is very awkward: Equations/Function/Program Fixpoint 
+  do not support mutual well-founded definitions. 
+  So we need this awkward encoding. Is there a way to make this
+  more generic?*)
+
+
+Definition size_l (A: Type) (l: list A) : nat :=
+  list_rect (fun _ => nat) 0 (fun _ _ rec => S rec) l.
+
+(*Now, for example, let us define functions that work on the size
+  of the list*)
+
+  Require Import Coq.Arith.Wf_nat.
+
+Section ListRectAlt.
+
+Variable A: Type.
+Variable P: list A -> Type.
+Variable P_lt: forall (l: list A) (IH:forall (x: list A), 
+  size_l _ x < size_l _ l -> P x), P l.
+
+Definition list_rect_alt (l: list A) : P l :=
+  Fix (well_founded_ltof _ (size_l A)) (fun l => P l) P_lt l.
+
+End ListRectAlt.
+(*
+(*Write functions on terms/formulas based on the smaller relation*)
+Section TermFmlaAlt.
+
+Variable P1: term -> Type.
+Variable P2: formula -> Type.
+Variable P_tm: forall (t2: term) (IH: forall (t1: term),
+  tm_size t1 < tm_size t2 -> P1 t1), P1 t2.
+Variable P_fmla: forall (f2: formula) (IH: forall (f1: formula),
+  fmla_size f1 < fmla_size f2 -> P2 f1), P2 f2.
+
+Definition tm_fmla := Either term formula.
+Definition tm_fmla_ty (x: tm_fmla) : Type :=
+  match x with
+  | Left t => P1 t
+  | Right f => P2 f
+  end.
+Definition tm_fmla_size (x: tm_fmla) : nat :=
+  match x with
+  | Left t => tm_size t
+  | Right f => fmla_size f
+  end.
+
+(*The body is not important*)
+Definition term_formula_rect_alt (t: term) (f: formula) : P1 t * P2 f :=
+let fn :=
+Fix (well_founded_ltof _ (tm_fmla_size)) tm_fmla_ty
+(fun x =>
+  match x as x' return 
+  (forall y, ltof tm_fmla tm_fmla_size y x' -> tm_fmla_ty y) ->
+  tm_fmla_ty x' with
+  | Left t => fun IH => P_tm t (fun t1 Hsz => IH (Left _ _ t1) Hsz)
+  | Right f => fun IH => P_fmla f (fun f1 Hsz => IH (Right _ _ f1) Hsz)
+  end) in
+(fn (Left _ _ t), fn (Right _ _ f)).
+
+End TermFmlaAlt.*)
+
+(*I think we should just do with Equations, we want this to be readable*)
+
+
+  (*
+  Context {A : Type} (f : A -> nat).
+  Equations list_size (l : list A) : nat :=
+   | nil := 0
+   | x :: xs := S (f x + list_size xs).
+  
+  Lemma In_list_size:
+    forall x xs, In x xs -> f x < S (list_size xs).
+  Proof.
+    intros. funelim (list_size xs); simpl in *. destruct H.
+    destruct H0.
+    * subst; lia.
+    * specialize (H _ H0). intuition. 
+  Qed.
+End list_size.
+Transparent list_size.
+
+Module RoseTree.
+
+  Section roserec.
+    Context {A : Set}.
+
+    Inductive t : Set :=
+    | leaf (a : A) : t
+    | node (l : list t) : t.
+    Derive NoConfusion for t.
+
+    Fixpoint size (r : t) :=
+      match r with
+      | leaf a => 0
+      | node l => S (list_size size l)
+      end.
+
+    Equations? elements (r : t) : list A by wf (size r) lt :=
+    elements (leaf a) := [a];
+    elements (node l) := concat (map_In l (fun x H => elements x)).
+    Proof. red. now apply In_list_size. Qed.
+      
+    Equations elements_def (r : t) : list A :=
+    elements_def (leaf a) := [a];
+    elements_def (node l) := concat (List.map elements_def l).
+    Lemma elements_equation (r : t) : elements r = elements_def r.
+    Proof.
+      funelim (elements r); simp elements_def; trivial. f_equal.
+      induction l; simpl; auto. simp map_In. rewrite H. rewrite IHl; auto.
+      intros. apply H. now constructor 2. now constructor.
+    Qed.
+
+    (** To solve measure subgoals *)
+    Hint Extern 4 (_ < _) => simpl; lia : Below.
+    Hint Extern 4 (MR _ _ _ _) => repeat red; simpl in *; lia : Below.
+
+    Obligation Tactic := simpl in *; program_simpl; try typeclasses eauto with Below subterm_relation.
+    (* Nested rec *) 
+
+
+*)
+Section ElimLet.
+
+Context (bt bf: bool).
+
+
+(*TODO: see*)
+
+(*Fixpoint elim_let_t (t: term) : term :=
+  match t with
+  | Tlet tm1 x tm2 => 
+    if bt then
+    safe_sub_t (elim_let_t tm1) x (elim_let_t tm2)
+    else Tlet (elim_let_t tm1) x (elim_let_t tm2)
+  | _ => t_map elim_let_t elim_let_f t
+  end 
+with elim_let_f (f: formula) : formula :=
+match f with
+| Flet tm1 x f => 
+  if bt then
+  safe_sub_f (elim_let_t tm1) x (elim_let_f f)
+  else Flet (elim_let_t tm1) x (elim_let_f f)
+| _ => f_map elim_let_t elim_let_f f
+end.*)
+
+(*For the Equations proofs, we need a map function
+  where we only prove the property for all elements in a list,
+  not any arbitrary element*)
+(*Fixpoint map_dep_in {A B: Type} (eq_dec: forall (x y: A), {x=y} +{x<>y}) 
+  (l: list A) (f: {x: A | in_bool eq_dec x l} -> B):
+  list B :=
+  match l as l' return ({x: A | in_bool eq_dec x l'} -> B) -> list B
+  with
+  | nil => fun _ => nil
+  | x :: t => fun f => f (exist _ x _) :: map_dep_in eq_dec t 
+    (fun y => f
+  end.
+
+Check dep_map.
+*)
+
+(*The [t_map] and [f_map] that Why3 uses does not work
+  with the wf measure here: we get impossible obligations,
+  where we need to show that arbitrary terms are smaller than
+  some fixed size*)
+
+Fixpoint times_free_t (x: vsymbol) (t: term) : nat :=
+  match t with
+  | Tfun _ _ tms => sum (map (times_free_t x) tms)
+  | Tlet t1 v t2 => times_free_t x t1 +
+    (if vsymbol_eq_dec x v then 0 else times_free_t x t2)
+  | Tif f t1 t2 => times_free_f x f + times_free_t x t1 + times_free_t x t2
+  | Tvar v => if vsymbol_eq_dec x v then 1 else 0
+  | Tconst _ => 0
+  | Teps f v => if vsymbol_eq_dec x v then 0 else times_free_f x f
+  | Tmatch t _ ps => times_free_t x t +
+    sum (map (fun p => if in_bool vsymbol_eq_dec x (pat_fv (fst p)) then
+      0 else times_free_t x (snd p)) ps)
+  end
+with times_free_f (x: vsymbol) (f: formula) : nat :=
+  match f with
+  | Fpred _ _ tms => sum (map (times_free_t x) tms)
+  | Fquant _ v f => if vsymbol_eq_dec x v then 0 else times_free_f x f
+  | Fbinop _ f1 f2 => times_free_f x f1 + times_free_f x f2
+  | Feq _ t1 t2 => times_free_t x t1 + times_free_t x t2
+  | Fnot f => times_free_f x f
+  | Flet t v f => times_free_t x t +
+    (if vsymbol_eq_dec x v then 0 else times_free_f x f)
+  | Fif f1 f2 f3 => times_free_f x f1 + times_free_f x f2 +
+    times_free_f x f3
+  | Fmatch t _ ps => times_free_t x t +
+    sum (map (fun p => if in_bool vsymbol_eq_dec x (pat_fv (fst p)) then
+      0 else times_free_f x (snd p)) ps)
+  | Ftrue => 0
+  | Ffalse => 0
+  end.
+
+
+Lemma times_free_t_in x t f:
+  ((times_free_t x t) = 0 <-> ~In x (tm_fv t)) /\
+  ((times_free_f x f) = 0 <-> ~In x (fmla_fv f)).
+Proof.
+  revert t f; apply term_formula_ind; simpl; intros; auto;
+  try solve[split; intros; auto].
+  - vsym_eq x v; split; intros; auto; try discriminate;
+    not_or Hv; try contradiction. intros [Hxv | []]; subst; 
+    contradiction.
+  - rewrite sum_0, Forall_map. split; intros.
+    + intro C. simpl_set.
+      destruct C as [y [Hy Hinx]].
+      rewrite Forall_forall in *.
+      specialize (H _ Hy).
+      specialize (H0 _ Hy).
+      apply H; auto.
+    + revert H. apply Forall_impl_strong; intros.
+      apply H1. intro C.
+      apply H0. simpl_set. exists a; auto.
+  - simpl_set. vsym_eq x v; simpl; split; intros; auto.
+    + intro C. destruct_all; auto; try contradiction.
+      apply H; auto; lia.
+    + not_or Hx. apply H in Hx. rewrite Hx; auto.
+    + intro C.
+      destruct_all; subst; [apply H | apply H0]; auto; try lia.
+    + not_or Hx. apply H in Hx.
+      assert (~ In x (tm_fv tm2)) by auto. apply H0 in H1. lia.
+Admitted.
+
+(*We prove a stronger lemma - the size of a substituted term
+  is equal to the size of the original term t plus
+  the size of the new term times the number of times x appears
+  free in t. We need this for a strong enough IH in the function/predicate
+  (and probably match) case*)
+(*Not sure we need thi*)
+Lemma tm_size_sub_t t1 x t f:
+  (tm_size (sub_t t1 x t) = tm_size t + (times_free_t x t) * (tm_size t1)) /\
+  (fmla_size (sub_f t1 x f) = fmla_size f +
+    (times_free_f x f) * (tm_size t1)).
+Proof.
+  revert t f; apply term_formula_ind; simpl; intros; auto; try lia.
+  - vsym_eq x v; simpl; try lia.
+  - induction l1; simpl in *; auto; try lia.
+    inversion H; subst.
+    apply IHl1 in H3; lia.
+  - rewrite H. vsym_eq x v; lia.
+  - rewrite H. f_equal.
+    rewrite <- !Nat.add_assoc. f_equal.
+    rewrite Nat.mul_add_distr_r, Nat.add_assoc,
+    (Nat.add_comm (sum _) (_* tm_size t1)), <- !Nat.add_assoc. 
+    f_equal. clear H.
+    (*Now we just have the recursive goal*)
+    induction ps; simpl in *; auto; try lia.
+    inversion H0; subst.
+    specialize (IHps H3).
+    destruct (in_bool vsymbol_eq_dec x (pat_fv (fst a))); simpl; auto; lia.
+  - vsym_eq x v; simpl; lia.
+  - induction tms; simpl in *; auto; try lia.
+    inversion H; subst.
+    apply IHtms in H3; lia.
+  - vsym_eq x v; simpl;lia.
+  - vsym_eq x v; simpl; lia.
+  - rewrite H. f_equal.
+    rewrite <- !Nat.add_assoc. f_equal.
+    rewrite Nat.mul_add_distr_r, Nat.add_assoc,
+    (Nat.add_comm (sum _) (_* tm_size t1)), <- !Nat.add_assoc. 
+    f_equal. clear H.
+    (*Now we just have the recursive goal*)
+    induction ps; simpl in *; auto; try lia.
+    inversion H0; subst.
+    specialize (IHps H3).
+    destruct (in_bool vsymbol_eq_dec x (pat_fv (fst a))); simpl; auto; lia.
+Qed.
+
+(*I am dumb - this is NOT smaller
+  What we need (or could use) is a lexicographic order:
+  (num_lets x, tm_size x)
+*)
+
+
+
+Definition tm_fmla_let (x: tm_fmla) : nat :=
+  match x with
+  | Left t => count_let_t t
+  | Right f => count_let_f f
+  end.
+
+(*Lexicographic order via nats - stdlib only has pairs*)
+Section Lex.
+
+Context {A: Type} (r1 r2: A -> nat).
+
+Inductive lex : A -> A -> Prop :=
+  | lex_fst: forall x y,
+    r1 x < r1 y ->
+    lex x y
+  | lex_snd: forall x y,
+    r1 x = r1 y ->
+    r2 x < r2 y ->
+    lex x y.
+
+(*Prove well-founded*)
+(*Is this true? yes*)
+
+Lemma r1_acc: forall x y,
+  r1 x < r1 y ->
+  Acc lex y ->
+  Acc lex x.
+Proof.
+  intros. generalize dependent x.
+  induction H0; simpl; intros.
+  assert (lex x0 x) by (constructor; auto).
+  apply H; auto.
+Qed.
+
+Lemma acc_r1_r2: forall (x: A),
+  Acc r1 x ->
+  ()
+
+End Lex.
+Require Import Coq.Relations.Relation_Operators.
+
+Section Foo.
+Import SigTNotations.
+
+  Variable A : Type.
+  Variable B : A -> Type.
+  Variable leA : A -> A -> Prop.
+  Variable leB : forall x : A, B x -> B x -> Prop.
+
+  Notation LexProd := (lexprod leA leB).
+
+  Lemma acc_A_B_lexprod :
+    forall x : A,
+      Acc leA x ->
+      (forall x0 : A, clos_trans A leA x0 x -> well_founded (leB x0)) ->
+      forall y : B x, Acc (leB x) y -> Acc LexProd (x; y).
+  Proof.
+    induction 1 as [x _ IHAcc]; intros H2 y.
+    induction 1 as [x0 H IHAcc0]; intros.
+    apply Acc_intro.
+    destruct y as [x2 y1]; intro H6.
+    simple inversion H6; intro.
+    - cut (leA x2 x); intros.
+      + apply IHAcc; auto with sets.
+        * intros.
+          apply H2.
+          apply t_trans with x2; auto with sets.
+
+        * red in H2.
+          apply H2.
+          auto with sets.
+
+      + injection H1 as [= <- _].
+        injection H3 as [= <- _]; auto with sets.
+
+    - rewrite <- H1.
+      apply eq_sigT_eq_dep in H3.
+      destruct H3.
+      apply IHAcc0.
+      assumption.
+  Defined.*)
+
+  Theorem wf_lexprod :
+    well_founded leA ->
+    (forall x : A, well_founded (leB x)) -> well_founded LexProd.
+  Proof.
+    intros wfA wfB; unfold well_founded.
+    destruct a.
+    apply acc_A_B_lexprod; auto with sets; intros.
+    red in wfB.
+    auto with sets.
+  Defined.
+
+Check wf_incl.
+
+Lemma lex_acc2: forall x y,
+  r1 x = r1 y ->
+  r2 x < r2 y ->
+  Acc lex x.
+Proof.
+  intros.
+  remember (r2 y) as n.
+  generalize dependent x.
+  generalize dependent y.
+  induction n; simpl; intros; auto; try lia.
+  constructor.
+  intros. inversion H1; subst.
+  - 
+
+(*
+Lemma lex_acc1: forall n x,
+  r1 x < n ->
+  Acc lex x.
+Proof.
+  induction n; simpl; intros; try lia.
+  constructor.
+  intros.
+  inversion H0; subst.
+  - apply IHn; lia.
+  - 
+
+  remember (r1 y) as n.
+  generalize dependent y.
+  generalize dependent x.
+  induction n; simpl; intros; subst; auto; try lia.
+  constructor.
+  intros. inversion H0; subst.
+  - 
+
+
+  - lia. constructor; intros.
+    + inversion H0; subst.
+  *)
+
+Lemma lex_acc: forall x,
+  Acc lex x.
+Proof.
+  intros.
+  constructor.
+  intros.
+  induction H.
+  - admit.
+  -  
+
+
+  remember (r1 x) as n1.
+  generalize dependent x.
+  induction n1; simpl; intros.
+  - constructor; intros.
+    inversion H; subst; auto; try lia.
+
+  - constructor; intros.
+    inversion H; subst.
+
+
+  remember (r1 x) as n1.
+  remember (r2 x) as n2.
+  
+  generalize dependent x.
+  
+  induction n1; simpl; intros.
+  - constructor. intros.
+    inversion H; subst.
+    + lia.
+    + 
+  assert (forall y, r1 y < r1 x -> Acc lex )
+
+Lemma lex_wf: well_founded lex.
+Proof.
+  unfold well_founded.
+  intros.
+  constructor.
+  intros.
+  induction H.
+
+
+
+Require Import Coq.Relations.Relation_Operators.
+Check well_founded_ltof.
+Check ltof.
+(*The relation we use*)
+Definition elim_let_rel: tm_fmla -> tm_fmla -> Prop :=
+  slexprod _ _ (ltof _ tm_fmla_let) (ltof _ tm_fmla_size).
+
+
+
+
+
+
+cbn.
+subst.
+
+
+simpl.
+
+
+lia.
+
+Search (?x < S ?y).
+
+in_sum_le
+
+
+
+Admitted.
+Next Obligation.
+Admitted.
+Next Obligation.
+Admitted.
+Next Obligation.
+Admitted.
+Next Obligation.
+
+Search elim_let_tm_fmla.
+
+
+(*Now we prove an induction principle *)
+
+
+
+elim_let_tm_fmla;.
+
+
+elim_let_tm_fmla (Left (Tconst c)) => Tconst c;
+elim_let_tm_fmla (Left (Tvar v)) => Tvar v;
+elim_let_tm_fmla (Left (Tfun f tys tms)) =>
+  Tfun f tys (map ((fun x => elim_let_tm_fmla (Left x))) tms);
+elim_let_tm_fmla (Left (Tlet tm1 x tm2)) =>
+  
+elim_let_tm_fmla (Left (Tif f t1 t2)) =>
+  Tif 
+  .
+
+
+
+(*Now we can define a function on sizes*)
+Definition elim_let_tm_fmla (t: term) (f: formula) :
+  term * formula :=
+  term_formula_rect_alt (fun _ => term) (fun _ => formula)
+  (fun t rec =>
+    match t with
+    | Tlet tm1 x tm2 => 
+    if bt then
+    rec (safe_sub_t (elim_let_t))
+
+
+    safe_sub_t (elim_let_t bt bf tm1) x (elim_let_t bt bf tm2)
+    else Tlet (elim_let_t bt bf tm1) x (elim_let_t bt bf tm2)
+  | Tfun f tys tms => Tfun f tys (map (elim_let_t bt bf) tms)
+  | Tif f t1 t2 =>
+    Tif (elim_let_f bt bf f) (elim_let_t bt bf t1)
+      (elim_let_t bt bf t2)
+  | Tmatch tm ty ps =>
+    Tmatch (elim_let_t bt bf tm) ty
+      (map (fun x => (fst x, elim_let_t bt bf (snd x))) ps)
+  | Teps f v =>
+    Teps (elim_let_f bt bf f) v
+  | _ => t
+    | 
+  
+  ).
+
+
+
+.
+
+
+
+  (fun x => match x with
+            ).
+
+
+Variable A: Type.
+
+
+Check list_rect_alt.
+
+
+
+Eval compute in (size_l _ [4;6;7;8]).
+
+
+Definition size (A: Type) (l: list A) : nat.
+induction l.
+exact 0.
+exact (S (IHl)).
+Show Proof.
+
+Definition size_l (A: Type) (l: list A) : nat :=
+  list_rect A (fun l => match l with | nil => 0 | _ :: t => )
+
+
+  Equations tm_fmla_func (x: tm_fmla) : tm_fmla_ret x
+  by wf (tm_fmla_size x) lt :=
+  tm_fmla_func (Left (Tconst c)) := tconst_case c;
+  tm_fmla_func (Left (Tvar v)) := tvar_case v;
+  tm_fmla_func (Left (Tfun f tys tms)) := tfun_case f tys 
+    (map (fun x => tm_fmla_func (Left _ _ x)) tms);
+  tm_fmla_func (Left (Tlet t1 v t2)) := 
+    tlet_case (tm_fmla_func (Left _ _ t1)) v (tm_fmla_func (Left _ _ t2));
+  tm_fmla_func (Left (Tif f t1 t2)) := tif_case f t1 t2;
+  tm_fmla_func (Left (Tmatch tm ty ps)) := tmatch_case tm ty ps;
+  tm_fmla_func (Left (Teps f v)) := teps_case f v;
+  tm_fmla_func (Right (Fpred p tys tms)) := fpred_case p tys tms;
+  tm_fmla_func (Right (Fquant q v f)) := fquant_case q v f;
+  tm_fmla_func (Right (Feq v t1 t2)) := feq_case v t1 t2;
+  tm_fmla_func (Right (Fbinop b f1 f2)) := fbinop_case b f1 f2;
+  tm_fmla_func (Right (Fnot f)) := fnot_case f;
+  tm_fmla_func (Right Ftrue) := ftrue_case;
+  tm_fmla_func (Right Ffalse) := ffalse_case;
+  tm_fmla_func (Right (Flet t v f)) := flet_case t v f;
+  tm_fmla_func (Right (Fif f1 f2 f3)) := fif_case f1 f2 f3;
+  tm_fmla_func (Right (Fmatch tm v ps)) := fmatch_case tm v ps
+  .
+
+
+
+
+Require Import Coq.Arith.Wf_nat.
+
+(*Equations/Function/Program Fixpoint do not support 
+  mutual well-founded definitions. So we give a custom utility
+  to do this for size*)
+Section SizeRec.
+
+Variable rec_term: forall t, 
+
+Variable tconst_case: constant -> term.
+Variable tvar_case: vsymbol -> term.
+Variable tfun_case: funsym -> list vty -> list term -> term.
+Variable tlet_case: term -> vsymbol -> term -> term.
+Variable tif_case: formula -> term -> term -> term.
+Variable tmatch_case: term -> vty -> list (pattern * term) -> term.
+Variable teps_case: formula -> vsymbol -> term.
+
+Variable fpred_case: predsym -> list vty -> list term -> formula.
+Variable fquant_case: quant -> vsymbol -> formula -> formula.
+Variable feq_case: vty -> term -> term -> formula.
+Variable fbinop_case: binop -> formula -> formula -> formula.
+Variable fnot_case: formula -> formula.
+Variable ftrue_case: formula.
+Variable ffalse_case: formula.
+Variable flet_case: term -> vsymbol -> formula -> formula.
+Variable fif_case: formula -> formula -> formula -> formula.
+Variable fmatch_case: term -> vty -> 
+  list (pattern * formula) -> formula.
+
+Definition tm_fmla := Either term formula.
+Definition tm_fmla_ret (x: tm_fmla) : Set :=
+  match x with
+  | Left _ => term
+  | Right _ => formula
+  end.
+
+Definition tm_fmla_size (x: tm_fmla) : nat :=
+  match x with
+  | Left t => tm_size t
+  | Right f => fmla_size f
+  end.
+
+Equations tm_fmla_func (x: tm_fmla) : tm_fmla_ret x
+  by wf (tm_fmla_size x) lt :=
+  tm_fmla_func (Left (Tconst c)) := tconst_case c;
+  tm_fmla_func (Left (Tvar v)) := tvar_case v;
+  tm_fmla_func (Left (Tfun f tys tms)) := tfun_case f tys 
+    (map (fun x => tm_fmla_func (Left _ _ x)) tms);
+  tm_fmla_func (Left (Tlet t1 v t2)) := 
+    tlet_case (tm_fmla_func (Left _ _ t1)) v (tm_fmla_func (Left _ _ t2));
+  tm_fmla_func (Left (Tif f t1 t2)) := tif_case f t1 t2;
+  tm_fmla_func (Left (Tmatch tm ty ps)) := tmatch_case tm ty ps;
+  tm_fmla_func (Left (Teps f v)) := teps_case f v;
+  tm_fmla_func (Right (Fpred p tys tms)) := fpred_case p tys tms;
+  tm_fmla_func (Right (Fquant q v f)) := fquant_case q v f;
+  tm_fmla_func (Right (Feq v t1 t2)) := feq_case v t1 t2;
+  tm_fmla_func (Right (Fbinop b f1 f2)) := fbinop_case b f1 f2;
+  tm_fmla_func (Right (Fnot f)) := fnot_case f;
+  tm_fmla_func (Right Ftrue) := ftrue_case;
+  tm_fmla_func (Right Ffalse) := ffalse_case;
+  tm_fmla_func (Right (Flet t v f)) := flet_case t v f;
+  tm_fmla_func (Right (Fif f1 f2 f3)) := fif_case f1 f2 f3;
+  tm_fmla_func (Right (Fmatch tm v ps)) := fmatch_case tm v ps
+  .
+Next Obligation.
+
+Definition tm_func (t: term) : term := tm_fmla_func (Left _ _ t).
+Definition fmla_func (f: formula) : formula := tm_fmla_func (Right _ _ f).
+
+Definition tm_fmla_funcs (t: term) (f: formula) : term * formula :=
+    (tm_func t, fmla_func f).
+
+  End SizeRec.
+
+Definition elim_let_tf (t: term) (f: formula) := tm_fmla_funcs.
+Check elim_let_tf.
+
+
+
+Definition tm_fmla_func_size (x: tm_fmla) : tm_fmla_ret x := 
+  Fix (well_founded_ltof _ tm_fmla_size) (fun x => tm_fmla_ret x)
+  (fun x =>
+    match x with
+    | Left (Tconst c) =>(tconst_case c)
+    | _ => Left tm_d
+    end
+  
+  
+  )
+
+
+  
+  
+  tm_fmla (fun x y => ltof (tm_fmla_size x) (tm_fmla_size y))
+    .
+
+
+
+
+Check term_formula_rect.
+
+
+
+
+
+Variable const_case: constant -> 
+
+
+
+
+
+
+
+
+Section ElimLet.
+
+Variable bt: bool.
+Variable bf: bool.
+
+Equations elim_let_t (t: term) : term
+ by wf (tm_size t) lt :=
+ elim_let_t (Tlet tm1 x tm2) :=
+  if bt then
+  elim_let_t (safe_sub_t (elim_let_t tm1) x tm2)
+  else Tlet (elim_let_t tm1) x (elim_let_t tm2);
+elim_let_t (Tif f t1 t2) :=
+  Tif (elim_let_f f) (elim_let_t t1) (elim_let_t t2);
+elim_let_t (Tconst c) := Tconst c;
+elim_let_t (Tvar v) := Tvar v;
+elim_let_t (Tfun f tys tms) :=
+  Tfun f tys (map (fun x => elim_let_t x) tms);
+with elim_let_f (f: formula) : formula
+by wf (fmla_size f) lt :=
+elim_let_f (Fpred ps tys tms) =>
+  Fpred ps tys (map (fun x => elim_let_t x) tms)
+
+  .
+
+Function elim_let_t (bt: bool) (bf: bool) (t: term) {measure (size t)} : term :=
+match t with
+  | Tlet tm1 x tm2 => 
+    if bt then
+    safe_sub_t (elim_let_t bt bf tm1) x (elim_let_t bt bf tm2)
+    else Tlet (elim_let_t bt bf tm1) x (elim_let_t bt bf tm2)
+  | Tfun f tys tms => Tfun f tys (map (elim_let_t bt bf) tms)
+  | Tif f t1 t2 =>
+    Tif (elim_let_f bt bf f) (elim_let_t bt bf t1)
+      (elim_let_t bt bf t2)
+  | Tmatch tm ty ps =>
+    Tmatch (elim_let_t bt bf tm) ty
+      (map (fun x => (fst x, elim_let_t bt bf (snd x))) ps)
+  | Teps f v =>
+    Teps (elim_let_f bt bf f) v
+  | _ => t
+  end
+with elim_let_f (bt: bool) (bf: bool) (f: formula) : formula :=
+  match f with
+  | Fpred ps tys tms => Fpred ps tys (map (elim_let_t bt bf) tms)
+  | Fquant q v f => Fquant q v (elim_let_f bt bf f)
+  | Feq ty t1 t2 => Feq ty (elim_let_t bt bf t1) (elim_let_t bt bf t2)
+  | Fbinop b f1 f2 => Fbinop b (elim_let_f bt bf f1) (elim_let_f bt bf f2)
+  | Fnot f => Fnot (elim_let_f bt bf f)
+  | Flet tm1 v f =>
+    if bf then
+    safe_sub_f (elim_let_t bt bf tm1) v (elim_let_f bt bf f)
+    else Flet (elim_let_t bt bf tm1) v (elim_let_f bt bf f)
+  | Fif f1 f2 f3 => Fif (elim_let_f bt bf f1) (elim_let_f bt bf f2)
+    (elim_let_f bt bf f3)
+  | Fmatch tm ty ps =>
+    Fmatch (elim_let_t bt bf tm) ty
+      (map (fun x => (fst x, elim_let_f bt bf (snd x))) ps)
+  | _ => f
+  end.
+
+
+
+    
+    Search safe_sub_t tm_fv.
+
+
+    Search tm_fv safe_sub_t.
+  (sublist (tm_fv (elim_let_t bt bf t)) (tm_fv t))
+  (forall ty (Hty: term_has_type gamma t ty),
+    term_has_type gamma (elim_let_t bt bf t) ty) /\
+  (forall (Hty: formula_typed gamma f), formula_typed gamma (elim_let_f bt bf f)).
+
+
+
+
+
+
+
+
+  match 
+  | Tmatch tm ty ps =>
+    Tmatch (elim_let_t tm fmla tm)
+
+    
+    sub_t tm1' (elim_let_t tm fmla tm2)
+
+
+    elim_let_t tm fmla 
+      (if tm then sub_t (elim_let_t tm fmla tm1) x tm2 else t)
+  | 
